\documentclass{article}
\usepackage{amsmath,amssymb,physics,xfrac,nicefrac}
\usepackage{standalone}
\usepackage[left=1.5cm,top=1.5cm,right=1.5cm,bottom=1.5cm]{geometry}

 
\title{Quantum Field Theory Problem Sets}
\author{John Bortins}
 
\begin{document}
 
\maketitle{}
 
\section*{Problem 9.1}


\[\qq*{Given the translation operator}\hat{U}(\vb{a})=e^{-\text{i}\vb{\hat{p}}\cdot\vb{a}}\implies\pdv{\hat{U}(\vb{a})}{\vb{a}}=-\text{i}\vb{\hat{p}}e^{-\text{i}\vb{\hat{p}}\cdot\vb{a}}\implies\vb{\hat{p}}=-\frac{1}{\text{i}}\pdv{\hat{U}(\vb{a})}{\vb{a}}e^{\text{i}\vb{\hat{p}}\cdot\vb{a}}
\]
\[\qq*{Hence the generators are given by}\vb{\hat{p}}=\eval{-\frac{1}{\text{i}}\pdv{\hat{U}(\vb{a})}{\vb{a}}}_{\vb{a}=0}\qquad\blacksquare
\] 
\section*{Problem 9.2}

\[\qq*{Given}K^1=\eval{\frac{1}{\text{i}}\pdv{\hat{D}(\phi^1)}{\phi^1}}_{\phi^1=0}\qq{and}
D(\phi^1)=\vb{\Lambda}(\phi^1)=\begin{pmatrix}
\cosh{\phi^1}&\sinh{\phi^1}&0&0\\
\sinh{\phi^1}&\cosh{\phi^1} & 0&0 \\ 
0 & 0&1&0\\
0&0&0&1
\end{pmatrix}
\]

\[K^1=\eval{\frac{1}{\text{i}}\pdv{\hat{D}(\phi^1)}{\phi^1}}_{\phi^1=0}=\eval{\frac{1}{\text{i}}\begin{pmatrix}
		\sinh{\phi^1}&\cosh{\phi^1}&0&0\\
		\cosh{\phi^1}&\sinh{\phi^1} & 0&0 \\ 
		0 & 0&0&0\\
		0&0&0&0
		\end{pmatrix}}_{\phi^1=0}=-\text{i}\begin{pmatrix}
		0&1&0&0\\
		1&0 & 0&0 \\ 
		0 & 0&0&0\\
		0&0&0&0
		\end{pmatrix}\qquad\blacksquare
\]
\[\qq*{Given}K^2=\eval{\frac{1}{\text{i}}\pdv{\hat{D}(\phi^2)}{\phi^2}}_{\phi^2=0}\qq{and}
D(\phi^2)=\vb{\Lambda}(\phi^2)=\begin{pmatrix}
\cosh{\phi^2}&0&\sinh{\phi^2}&0\\
0&1 & 0&0 \\ 
\sinh{\phi^2} & 0&\cosh{\phi^2}&0\\
0&0&0&1
\end{pmatrix}
\]
\[\qq*{Clearly,}K^2=-\text{i}\begin{pmatrix}
		0&0&1&0\\
		0 & 0&0&0\\
		1&0 & 0&0 \\ 
		0&0&0&0
		\end{pmatrix}\qquad\blacksquare
\]



\[\qq*{Given}K^3=\eval{\frac{1}{\text{i}}\pdv{\hat{D}(\phi^3)}{\phi^3}}_{\phi^3=0}\qq{and}
D(\phi^3)=\vb{\Lambda}(\phi^3)=\begin{pmatrix}
\cosh{\phi^3}&0&0&\sinh{\phi^3}\\
0&1 & 0&0 \\ 
0 & 0&1&0\\
\sinh{\phi^3}&0&0&\cosh{\phi^3}
\end{pmatrix}
\]
\[\qq*{Clearly,}K^3=-\text{i}\begin{pmatrix}
		0&0&0&1\\
		0 & 0&0&0\\
		0&0&0&0 \\
		1&0 & 0&0 
		\end{pmatrix}\qquad\blacksquare
\] 
\section*{Problem 9.3}
\[D(\vb{\phi})=e^{\text{i}\vb{K}\cdot\vb{\phi}}\approx 1+\text{i}\vb{K}\cdot\vb{\phi}
\]




\[\omega^{\mu\nu}={\omega^\mu}_\lambda g^{\lambda\nu}=\begin{pmatrix}0&v^1&v^2&v^3\\v^1&0&\theta^3&-\theta^2\\v^2&-\theta^3&0&\theta^1\\v^3&\theta^2&-\theta^1&0\end{pmatrix}
\begin{pmatrix}1&0&0&0\\0&-1&0&0\\0&0&-1&0\\0&0&0&-1\end{pmatrix}=
\begin{pmatrix}0&-v^1&-v^2&-v^3\\v^1&0&-\theta^3&\theta^2\\v^2&\theta^3&0&-\theta^1\\v^3&-\theta^2&\theta^1&0\end{pmatrix}\]

\[\omega_{\mu\nu}=g_{\mu\lambda}{\omega^\lambda}_\nu =\begin{pmatrix}1&0&0&0\\0&-1&0&0\\0&0&-1&0\\0&0&0&-1\end{pmatrix}
\begin{pmatrix}0&v^1&v^2&v^3\\v^1&0&\theta^3&-\theta^2\\v^2&-\theta^3&0&\theta^1\\v^3&\theta^2&-\theta^1&0\end{pmatrix}=
\begin{pmatrix}0&v^1&v^2&v^3\\-v^1&0&-\theta^3&\theta^2\\-v^2&\theta^3&0&-\theta^1\\-v^3&-\theta^2&\theta^1&0\end{pmatrix}\]

Clearly the transposes of the resultant matrices are the negatives of the resultant matrices. Hence the resultant matrices are skew-symmetric, which is otherwise known as antisymmetric.


 
\section*{Problem 9.4}

Given \[ f(x^\prime) = f(x)+a^\mu \partial_\mu f(x)+{\omega^\mu}_\nu x^\nu \partial_\mu f(x)\] we know these things \[\omega^{\mu\nu}={\omega^\mu}_\lambda g^{\lambda\nu} \] and \[\omega_{\mu\nu}= g_{\mu\lambda} {\omega^\lambda}_\nu \] and \[g^{\mu\lambda}g_{\lambda\nu} = I\] and \[A_\mu=g_{\mu\nu}A^\nu\] and \[A^\mu=g^{\mu\nu}A_\nu\] and \[{\omega^\mu}_\nu=\frac{1}{2}[{\omega^\mu}_\nu+{{\omega^\mu}_\nu}^T]+\frac{1}{2}[{\omega^\mu}_\nu-{{\omega^\mu}_\nu}^T]=\frac{1}{2}[{\omega^\mu}_\nu+{\omega_\mu}^\nu]+\frac{1}{2}[{\omega^\mu}_\nu-{\omega_\mu}^\nu]\]

Examine \[{\omega^\mu}_\nu x^\nu \partial_\mu=\sum^3_{\mu=0}\sum^3_{\nu=0}{\omega^\mu}_\nu x^\nu \partial_\mu\]
\begin{multline*}
{\omega^\mu}_\nu x^\nu \partial_\mu=
v^1 x^1 \partial_0+v^2 x^2 \partial_0+v^3 x^3 \partial_0+
v^1 x^0 \partial_1+\theta^3 x^2 \partial_1-\theta^2 x^3 \partial_1\\+ 
v^2 x^0 \partial_2-\theta^3 x^1 \partial_2+\theta^1 x^3 \partial_2+
v^3 x^0 \partial_3+\theta^2 x^1 \partial_3-\theta^1 x^2 \partial_3
\end{multline*}

Examine \[\omega_{\mu\nu} (x^\mu \partial^\nu-x^\nu \partial^\mu)=\sum^3_{\mu=0}\sum^3_{\nu=0}\omega_{\mu\nu} x^\mu \partial^\nu-\sum^3_{\mu=0}\sum^3_{\nu=0}\omega_{\mu\nu} x^\nu \partial^\mu\]
\begin{multline*}
\omega_{\mu\nu} (x^\mu \partial^\nu-x^\nu \partial^\mu)=
v^1 x^0 \partial^1+v^2 x^0 \partial^2+v^3 x^0 \partial^3
-v^1 x^1 \partial^0-\theta^3 x^1 \partial^2+\theta^2 x^1 \partial^3\\ 
-v^2 x^2 \partial^0+\theta^3 x^2 \partial^1-\theta^1 x^2 \partial^3
-v^3 x^3 \partial^0-\theta^2 x^3 \partial^1+\theta^1 x^3 \partial^2\\-
(v^1 x^1 \partial^0+v^2 x^2 \partial^0+v^3 x^3 \partial^0
-v^1 x^0 \partial^1-\theta^3 x^2 \partial^1+\theta^2 x^3 \partial^1\\ 
-v^2 x^0 \partial^2+\theta^3 x^1 \partial^2-\theta^1 x^3 \partial^2
-v^3 x^0 \partial^3-\theta^2 x^1 \partial^3+\theta^1 x^2 \partial^3)\end{multline*}
\begin{multline*}
\omega_{\mu\nu} (x^\mu \partial^\nu-x^\nu \partial^\mu)=
v^1 x^0 \partial^1+v^2 x^0 \partial^2+v^3 x^0 \partial^3
-v^1 x^1 \partial^0-\theta^3 x^1 \partial^2+\theta^2 x^1 \partial^3\\ 
-v^2 x^2 \partial^0+\theta^3 x^2 \partial^1-\theta^1 x^2 \partial^3
-v^3 x^3 \partial^0-\theta^2 x^3 \partial^1+\theta^1 x^3 \partial^2\\
-v^1 x^1 \partial^0-v^2 x^2 \partial^0-v^3 x^3 \partial^0
+v^1 x^0 \partial^1+\theta^3 x^2 \partial^1-\theta^2 x^3 \partial^1\\ 
+v^2 x^0 \partial^2-\theta^3 x^1 \partial^2+\theta^1 x^3 \partial^2
+v^3 x^0 \partial^3+\theta^2 x^1 \partial^3-\theta^1 x^2 \partial^3\end{multline*}

But $\partial^i=-\partial_i$ and $\partial^0=\partial_0$, therefore
\begin{multline*}
\omega_{\mu\nu} (x^\mu \partial^\nu-x^\nu \partial^\mu)=
-v^1 x^0 \partial_1-v^2 x^0 \partial_2-v^3 x^0 \partial_3
-v^1 x^1 \partial_0+\theta^3 x^1 \partial_2-\theta^2 x^1 \partial_3\\ 
-v^2 x^2 \partial_0-\theta^3 x^2 \partial_1+\theta^1 x^2 \partial_3
-v^3 x^3 \partial_0+\theta^2 x^3 \partial_1-\theta^1 x^3 \partial_2\\
-v^1 x^1 \partial_0-v^2 x^2 \partial_0-v^3 x^3 \partial_0
-v^1 x^0 \partial_1-\theta^3 x^2 \partial_1+\theta^2 x^3 \partial_1\\ 
-v^2 x^0 \partial_2+\theta^3 x^1 \partial_2-\theta^1 x^3 \partial_2
-v^3 x^0 \partial_3-\theta^2 x^1 \partial_3+\theta^1 x^2 \partial_3\end{multline*}

Finally
\[{\omega^\mu}_\nu x^\nu \partial_\mu=-\frac{1}{2}\omega_{\mu\nu} (x^\mu \partial^\nu-x^\nu \partial^\mu)\]

\end{document}