\documentclass{article}
\usepackage{amsmath,amssymb,physics,xfrac,nicefrac}
\usepackage{standalone}
\usepackage[left=1.5cm,top=1.5cm,right=1.5cm,bottom=1.5cm]{geometry}

 
\title{Quantum Field Theory Problem Sets}
\author{John Bortins}
 
\begin{document}
 
\maketitle{}

\section*{Notes}

Time dependence in operators (Heisenberg) and time dependence in wave functions (Schr\"odinger). Preserving special relativity.
 
\section*{Problem 8.1} 

\[\qq*{Given the time evolution operator} \hat{U}(t_2,t_1)=\exp[-\text{i}\hat{H}(t_2-t_1)] \]
 
\[\qq*{Property 1:} \hat{U}(t_1,t_1)=e^{-\text{i}\hat{H}(t_1-t_1)}=e^{0}=1\qquad\blacksquare \]

\begin{align*}
\qq*{Property 2:} \hat{U}(t_3,t_2)\hat{U}(t_2,t_1)&=e^{-\text{i}\hat{H}(t_3-t_2)}e^{-\text{i}\hat{H}(t_2-t_1)}\\
&=e^{-\text{i}\hat{H}[(t_3-t_2)+(t_2-t_1)]}\\
&=e^{-\text{i}\hat{H}(t_3-t_1)}=\hat{U}(t_3,t_1)\qquad\blacksquare 
\end{align*}

\begin{align*}
\qq*{Property 3:} \text{i}\dv{t_2}\hat{U}(t_2,t_1)&=\text{i}\dv{t_2}e^{-\text{i}\hat{H}(t_2-t_1)}\\
&=\text{i}e^{-\text{i}\hat{H}(t_2-t_1)}(-\text{i}\hat{H}) \\
&=\hat{H}e^{-\text{i}\hat{H}(t_2-t_1)}=\hat{H}\hat{U}(t_2,t_1) \qquad\blacksquare 
\end{align*}
 

\[\qq*{Property 4:} \hat{U}(t_1,t_2)=e^{-\text{i}\hat{H}(t_1-t_2)}=e^{-\text{i}\hat{H}(t_2-t_1)(-1)}=\hat{U}^{-1}(t_2,t_1)\qquad\blacksquare \]

\begin{align*}
\qq*{Property 5:} \hat{U}^{\dagger}(t_2,t_1)\hat{U}(t_2,t_1)&=\qty[e^{-\text{i}\hat{H}(t_2-t_1)}]^{\dagger} e^{-\text{i}\hat{H}(t_2-t_1)}\\
&=e^{+\text{i}\hat{H}(t_2-t_1)}e^{-\text{i}\hat{H}(t_2-t_1)}=1 \qquad\blacksquare 
\end{align*}
 

\section*{Problem 8.2}
 
\[\qq*{Given} \hat{H}=\sum_k E_k \hat{a}_k^\dagger \hat{a}_k \] 
\[\qq*{Recall} \qty[a,a^\dagger]=1\]
\begin{align*}
\text{i}\hbar\dv{\hat{a}_k^\dagger }{t}&= \qty[\hat{a}_k^\dagger ,\hat{H}]\\
&=\hat{a}_k^\dagger E_{k}\hat{a}_k^\dagger\hat{a}_k-E_{k}\hat{a}_k^\dagger\hat{a}_k\hat{a}_k^\dagger \\
&=\hat{a}_k^\dagger E_{k}\qty(\hat{a}_k\hat{a}_k^\dagger-1)-E_{k}\hat{a}_k^\dagger\hat{a}_k\hat{a}_k^\dagger =-E_{k}\hat{a}_k^\dagger 
\end{align*}

\begin{align*}
\text{i}\hbar\int\frac{\dd{\hat{a}_k^\dagger }}{\hat{a}_k^\dagger}&=-E_{k}\int\dd{t} \\
\ln{\hat{a}_k^\dagger(t)}-\ln{\hat{a}_k^\dagger(0)}&=-\frac{E_{k}}{\text{i}\hbar}t \\
\hat{a}_k^\dagger(t)&=\hat{a}_k^\dagger(0)e^{\nicefrac{\text{i}tE_{k}}{\hbar}}\qquad\blacksquare 
\end{align*}

\begin{align*}
\qq*{Similarly} \text{i}\hbar\dv{\hat{a}_k }{t}&= \qty[\hat{a}_k ,\hat{H}]\\
&=\hat{a}_k E_{k}\hat{a}_k^\dagger\hat{a}_k-E_{k}\hat{a}_k^\dagger\hat{a}_k\hat{a}_k \\
&=\hat{a}_k E_{k}\hat{a}_k^\dagger\hat{a}_k-E_{k}(\hat{a}_k\hat{a}_k^\dagger-1)\hat{a}_k =E_{k}\hat{a}_k
\end{align*}

\begin{align*}
\text{i}\hbar\int\frac{\dd{\hat{a}_k }}{\hat{a}_k}&=E_{k}\int\dd{t} \\
\ln{\hat{a}_k(t)}-\ln{\hat{a}_k(0)}&=\frac{E_{k}}{\text{i}\hbar}t \\
\hat{a}_k(t)&=\hat{a}_k(0)e^{\nicefrac{-\text{i}tE_{k}}{\hbar}}\qquad\blacksquare 
\end{align*}


\section*{Problem 8.3}

\[\qq*{Given} \hat{X}= X_{lm}\hat{a}_l^\dagger\hat{a}_m\qq{and}\hat{H}=\sum_k E_k \hat{a}_k^\dagger \hat{a}_k\] 
\[\qq*{Recall} \qty[a_i,a_j^\dagger]=\delta_{ij}\qq{,}\qty[a_i^\dagger,a_j^\dagger]=0\qq{and}\qty[a_i,a_j]=0\]

\begin{align*}
\text{i}\hbar\dv{\hat{X} }{t}&= \qty[\hat{X} ,\hat{H}]\\
&=X_{lm}\hat{a}_l^\dagger\hat{a}_m E_{l}\hat{a}_l^\dagger\hat{a}_l-E_{l}\hat{a}_l^\dagger\hat{a}_l X_{lm}\hat{a}_l^\dagger\hat{a}_m + X_{lm}\hat{a}_l^\dagger\hat{a}_m E_{m}\hat{a}_m^\dagger\hat{a}_m-E_{m}\hat{a}_m^\dagger\hat{a}_m X_{lm}\hat{a}_l^\dagger\hat{a}_m \\
&=X_{lm}E_{l}\hat{a}_l^\dagger\hat{a}_m \hat{a}_l^\dagger\hat{a}_l-X_{lm}E_{l}\hat{a}_l^\dagger\hat{a}_l \hat{a}_l^\dagger\hat{a}_m + X_{lm}E_{m}\hat{a}_l^\dagger\hat{a}_m \hat{a}_m^\dagger\hat{a}_m-X_{lm}E_{m}\hat{a}_m^\dagger\hat{a}_m \hat{a}_l^\dagger\hat{a}_m \\
&=X_{lm}E_{l}\hat{a}_l^\dagger\hat{a}_m \qty(\hat{a}_l\hat{a}_l^\dagger-1)-X_{lm}E_{l}\hat{a}_l^\dagger\hat{a}_l \hat{a}_l^\dagger\hat{a}_m + X_{lm}E_{m}\hat{a}_l^\dagger\hat{a}_m \hat{a}_m^\dagger\hat{a}_m-X_{lm}E_{m}\hat{a}_m^\dagger\hat{a}_m \hat{a}_l^\dagger\hat{a}_m \\
&=-X_{lm}E_{l}\hat{a}_l^\dagger\hat{a}_m+X_{lm}E_{l}\hat{a}_l^\dagger\hat{a}_m \hat{a}_l\hat{a}_l^\dagger-X_{lm}E_{l}\hat{a}_l^\dagger\hat{a}_l \hat{a}_l^\dagger\hat{a}_m + X_{lm}E_{m}\hat{a}_l^\dagger\hat{a}_m \hat{a}_m^\dagger\hat{a}_m-X_{lm}E_{m}\hat{a}_m^\dagger\hat{a}_m \hat{a}_l^\dagger\hat{a}_m \\
&=-X_{lm}E_{l}\hat{a}_l^\dagger\hat{a}_m + X_{lm}E_{m}\hat{a}_l^\dagger\hat{a}_m \hat{a}_m^\dagger\hat{a}_m-X_{lm}E_{m}\hat{a}_m^\dagger\hat{a}_m \hat{a}_l^\dagger\hat{a}_m \\
&=-X_{lm}E_{l}\hat{a}_l^\dagger\hat{a}_m + X_{lm}E_{m}\hat{a}_l^\dagger\hat{a}_m \hat{a}_m^\dagger\hat{a}_m-X_{lm}E_{m}(\hat{a}_m\hat{a}_m^\dagger-1) \hat{a}_l^\dagger\hat{a}_m \\
&=-X_{lm}E_{l}\hat{a}_l^\dagger\hat{a}_m + X_{lm}E_{m}\hat{a}_l^\dagger\hat{a}_m \hat{a}_m^\dagger\hat{a}_m-X_{lm}E_{m}\hat{a}_m \hat{a}_m^\dagger \hat{a}_l^\dagger \hat{a}_m+ X_{lm}E_{m}\hat{a}_l^\dagger\hat{a}_m \\
&=-E_{l}\hat{X}+E_{m}\hat{X}
\end{align*}

\begin{align*}
\text{i}\hbar\int\frac{\dd{\hat{X}}}{\hat{X}}&=\qty(-E_{l}+E_{m})\int\dd{t} \\
\ln{\hat{X}(t)}-\ln{\hat{X}(0)}&=\frac{-\qty(E_{l}-E_{m})}{\text{i}\hbar}t \\
\hat{X}(t)&=\hat{X}(0)e^{\nicefrac{\text{i}t\qty(E_{l}-E_{m})}{\hbar}}\qquad\blacksquare 
\end{align*}


\section*{Problem 8.4}

\[\qq*{Given} \hat{H}=\omega \hat{S}_y \] 

Recall XYZZY: $a_x=a_y a_z - a_z a_y$.

\begin{align*}
\text{i}\hbar\dv{\hat{S}_{z} }{t}&= \qty[\hat{S}_{z} ,\omega \hat{S}_y]\\
&=\hat{S}_{z}\omega \hat{S}_y-\omega \hat{S}_y \hat{S}_{z}\\
&=-\omega\qty(\hat{S}_y \hat{S}_{z}-\hat{S}_{z} \hat{S}_y)\\
&=-\text{i}\hbar\omega\hat{S}_x\\
\dv{\hat{S}_{z} }{t}&=-\omega\hat{S}_x\qquad\blacksquare 
\end{align*}

\begin{align*}
\text{i}\hbar\dv{\hat{S}_{x} }{t}&= \qty[\hat{S}_{x} ,\omega \hat{S}_y]\\
&=\hat{S}_{x}\omega \hat{S}_y-\omega \hat{S}_y \hat{S}_{x}\\
&=\omega\qty(\hat{S}_{x} \hat{S}_y-\hat{S}_y \hat{S}_{x})\\
&=\text{i}\hbar\omega\hat{S}_z\\
\dv{\hat{S}_{x} }{t}&=\omega\hat{S}_z\qquad\blacksquare 
\end{align*}


\begin{align*}
\qq*{Consider} \dv{\hat{S}_{x} }{t}&= \omega\hat{S}_z\\ 
\dv[2]{\hat{S}_{x} }{t}&= \omega\dv{\hat{S}_z}{t}\\ 
&= -\omega^2 \hat{S}_x\\
\dv[2]{\hat{S}_{x} }{t}+\omega^2 \hat{S}_x&=0\\
\qq*{Similarly}\dv[2]{\hat{S}_{z} }{t}+\omega^2 \hat{S}_z&=0
\end{align*}
That is to say, simple harmonic motion.$\qquad\blacksquare $ 



\end{document}