\documentclass{memoir}
\usepackage{graphicx,float}
\usepackage{amsmath,amssymb,xfrac,nicefrac}
\usepackage[left=1.5cm,top=1.5cm,right=1.5cm,bottom=1.5cm]{geometry}
\usepackage[italicdiff]{physics}
\usepackage{tikz}
\usetikzlibrary{arrows,shapes,positioning}
\usetikzlibrary{decorations.markings}
\tikzstyle arrowstyle=[scale=1]
\tikzstyle directed=[postaction={decorate,decoration={markings,
    mark=at position .65 with {\arrow[arrowstyle]{stealth}}}}]
\tikzstyle reverse directed=[postaction={decorate,decoration={markings,
    mark=at position .65 with {\arrowreversed[arrowstyle]{stealth};}}}]
 
\title{Quantum Field Theory Problem Sets}
\author{John Bortins}
 
\begin{document}

\maketitle{}

\section*{Notes}

Chapter 0 introduces the idea of a field in space and time. Other ideas are special relativity, sensible coordinate transformations, Einstein summation, the metric tensor, Fourier transforms and the Maxwell equations.

Chapter 1 talks about Fermat's principle of least time, functionals, Lagrangians, Hamilton's principle of least action, the Euler-Lagrange equation and the Lagrangian density.

\section*{Problem 1.1}

    \begin{tikzpicture}[>=stealth]

        % define coordinates
        \coordinate (O) at (0,0) ;
        \coordinate (A) at (0,4) ;
        \coordinate (B) at (0,-4) ;

        % media
        \fill[blue!5!] (-5,0) rectangle (5,4);
        \fill[blue!15!] (-5,0) rectangle (5,-4);
        \node[right] at (2,2) {Air};
        \node[left] at (-2,-2) {Water};

        % vertical axis
        \draw[dash pattern=on5pt off3pt] (A) -- (B) ;
        \node[right] at (0,3.5) {Normal through $(x,y)$};

        % rays
        \draw[red,ultra thick,reverse directed] (O) -- (130:4);
        \draw[blue,directed,ultra thick] (O) -- (-60:3);
        \node[below left] at (130:2)  {$L_1$};
        \node[above right] at (-60:1.5)  {$L_2$};

        % horizontals
        \draw[red,thick,<->]  (130:4)--(130:4 -| 0,0) node [midway,draw,fill=blue!5!] {$x-a$};
        \draw[blue,thick,<->] (-60:3)--(0,0 |- -60:3) node [midway,draw,fill=blue!15!] {$c-x$};

        % points
        \draw [red,fill] (130:4) circle [radius=0.075];
        \draw [blue,fill] (-60:3) circle [radius=0.075];
        \draw [fill] (0,0) circle [radius=0.075];
        \node[left] at (130:4)  {$(a,b)$};
        \node[right] at (-60:3)  {$(c,d)$};
        \node[above right] at (0,0)  {$(x,y)$};


        % angles
        \draw (0,1) arc (90:130:1);
        \draw (0,-1.4) arc (270:300:1.4) ;
        \node[] at (285:1.8)  {$\theta_{2}$};
        \node[] at (110:1.4)  {$\theta_{1}$};

        \node [below right, text width=8cm,align=justify] at (5.25,4) {
            For a ray of light from inside an area to inside another area. Let $(a,b)$ be the source. Let $(x,y)$ be at the interface. Let $(c,d)$ be the destination.\par
            Distance traveled is then $L_1=\sqrt {(a-x)^2+(b-y)^2}$ plus $L_2=\sqrt {(c-x)^2+(d-y)^2}$.\par
            Inside the upper area let the speed of light be $v_1$ and inside the lower area let the speed of light be $v_2$. The total time is then  \[T=\frac{\sqrt {(a-x)^2+(b-y)^2} } {v_1}+\frac{\sqrt {(c-x)^2+(d-y)^2} } {v_2}\]
            The only variable that will affect the total time $T$ is $x$. Recall that index of refraction $n$ is related to the speed of light $c$ and the velocity of light in the medium $v$ by $nv=c$.
            };



    \end{tikzpicture}

\[\dv {T} {x} = \frac{x-a}{v_1\sqrt {(a-x)^2+(b-y)^2}} - \frac{c-x}{v_2\sqrt {(c-x)^2+(d-y)^2}}=0  \]
\[\frac{x-a}{v_1 L_1} = \frac{c-x}{v_2 L_2}  \]
\[\qq*{Recognize the fractions as sines of angles} \frac{\sin \theta_1}{v_1} = \frac{\sin \theta_2}{v_2} \qor n_1 sin \theta_1 = n_2 \sin \theta_2\qquad \blacksquare\]




\section*{Problem 1.2}

A functional is defined by a rule that associates a number with a set of functions.
\[\qq*{For the set of functions}f_1, f_2, \cdots\qq{ this}\underrightarrow{rule}\qq{produces a number represented by} F[f_1, f_2].\]

The calculation of a functional derivative using test function $\delta(x)$ may be found from
\[\frac{\delta F[f(x)]}{\delta f(x_1)}=\lim_{\epsilon\to 0}\frac{F[f(x)-\epsilon\delta(x-x_1)]-F[f(x)]}{\epsilon}.    \]

A functional derivative is a functional of a functional, i.e.,
\[\var{G[f][h]}=\dv{\epsilon}G[f+\epsilon h]\Big\vert_{\epsilon=0}.\]


\begin{align*}
    \qq*{\S}\qq{Given}H[f]          & =\int G(x,y)f(y)dy\qq{find}\frac{\delta H[f]}{\delta f(z)}.                  \\
    \fdv{H[f]}{f(z)}&=\lim_{\epsilon\to 0}\frac{H[f(x)-\epsilon\delta(x-z)]-H[f(x)]}{\epsilon} \\
    &=\lim_{\epsilon\to 0}\frac{1}{\epsilon}\bqty{\int G(x,y)\bqty{f(y)+\epsilon\delta(y-z)}dy-\int G(x,y)f(y)dy}\\
    &=\lim_{\epsilon\to 0}\frac{1}{\epsilon}\bqty{\int G(x,y)f(y)+\epsilon\int G(x,y)\delta(y-z)dy-\int G(x,y)f(y)dy}\\
    &=\lim_{\epsilon\to 0}\int G(x,y)\delta(y-z)dy =G(x,z) \qq{where $z$ is within the limits of the integration}\\
\end{align*}


\begin{align*}
    \delta H[f][h]                  & =\frac{d}{d\epsilon}H[f+\epsilon h]\Big\vert_{\epsilon=0}                   \\
                                    & =\frac{d}{d\epsilon}\int G(x,y)(f(y)+\epsilon h(y))dy\Big\vert_{\epsilon=0} \\
                                    & =\int G(x,y)h(y)dy                                                          \\
                                    & =\int G(x,y)\delta(y-z)dy                                                   \\
    \frac{\delta H[f]}{\delta f(z)} & =G(x,z) \qq{where $z$ is within the limits of the integration} \blacksquare\\
\end{align*}

\begin{align*}
    \qq*{\S}\qq{Given}I[f] & =\int_{-1}^{1} f(x)dx\qq{find}\frac{\delta^2 I[f^3]}{\delta f(x_0)\delta f(x_1)}                                                   \\
    \delta I[f^3][h]       & =\frac{d}{d\epsilon}\int_{-1}^{1} (f(x)+\epsilon h(x))^3 dx\Big\vert_{\epsilon=0}                                                  \\
                           & =\frac{d}{d\epsilon}\int_{-1}^{1} [f(x)^3+3\epsilon f(x)^2 h(x)+3\epsilon^2 f(x)h(x)^2+\epsilon^3 h(x)^3] dx\Big\vert_{\epsilon=0} \\
                           & =\int_{-1}^{1} [3f(x)^2 h(x)+6\epsilon f(x)h(x)^2+3\epsilon^2 h(x)^3] dx\Big\vert_{\epsilon=0}                                     \\
                           & =\int_{-1}^{1} 3f(x)^2 h(x) dx                                                                                                     \\
\end{align*}


Now we do it again
\begin{align*}
    \delta \delta I[f^3][h][k]                              & =\frac{d}{d\epsilon}\int_{-1}^{1} 3(f(x)+\epsilon k(x))^2 h(x) dx\Big\vert_{\epsilon=0}                        \\
                                                            & =\frac{d}{d\epsilon}\int_{-1}^{1} 3[f(x)^2+2\epsilon f(x)k(x)+\epsilon^2 k(x)^2] h(x) dx\Big\vert_{\epsilon=0} \\
                                                            & =\int_{-1}^{1} 6f(x)k(x)h(x) dx                                                                                \\
    \frac{\delta \delta I[f^3]}{\delta f(x_0)\delta f(x_1)} & =\int_{-1}^{1} 6f(x)\delta(x-x_1)\delta(x-x_0) dx                                                              \\
                                                            & =6f(x_0)\delta(x_0-x_1)\qq{where}  -1\leq x_0, x_1\leq 1 \qquad \blacksquare                                   \\
\end{align*}


\begin{align*}
    \qq*{\S}\qq{Given}J[f] & =\int \left(\frac{\delta f}{\delta y}\right)^2 dy\qq{find}\frac{\delta J[f]}{\delta f(x)}               \\
    \delta J[f][h]         & =\frac{d}{d\epsilon}J[f+\epsilon h]\Big\vert_{\epsilon=0}                                               \\
                           & =\frac{d}{d\epsilon}\int \left(\frac{\delta (f+\epsilon h)}{\delta y}\right)^2 dy                       \\
                           & =\frac{d}{d\epsilon}\int \left(\frac{\delta f}{\delta y}+\epsilon\frac{\delta h}{\delta y} \right)^2 dy \\
                           & =2\int \frac{\delta f}{\delta y}\frac{\delta h}{\delta y}  dy                                           \\
\end{align*}

\begin{align*}
    \qq*{Consider the product rule }(u'v)'            & =u''v+u'v' \qq{where} u'=\frac{\delta f}{\delta y}\qand v=h                    \\
    \delta J[f][h]                  & =2\int\frac{\delta}{\delta y}\left(\frac{\delta f}{\delta y}h\right)dy-2\int\frac{\delta^2 f}{\delta y^2}h dy \\
                                    & =2\frac{\delta f}{\delta y}h\Big\vert_a^b-2\int\frac{\delta^2 f}{\delta y^2}h dy                              \\
                                    & =2\frac{\delta f}{\delta y}\delta(x-y)\Big\vert_a^b-2\int\frac{\delta^2 f}{\delta y^2}\delta(x-y) dy          \\
    \frac{\delta J[f]}{\delta f(x)} & =-2\frac{\delta^2 f}{\delta x^2}\qq*{where}  a<x<b \qquad \blacksquare                                        \\
\end{align*}

\[\]

\section*{Problem 1.3}
 \[\S\qq{Given}G[f]=\int g(y,f)dy\]
show that \[\frac{\delta G[f]}{\delta f(x)}=\frac{\partial g(x,f)}{\partial f} \]
\[\delta G[f][h]=\frac{d}{d\epsilon}G[f+\epsilon h]\Big\vert_{\epsilon=0}\]
\[\delta G[f][h]=\frac{d}{d\epsilon}\int g(y,f+\epsilon h)dy\]
Say \[g(y,f+\epsilon h)=g(y,f)+\frac{1}{1!}\frac{\partial g(y,f)}{\partial f}(\epsilon h) + \cdots \]
\[\delta G[f][h]=\int\frac{\partial g(y,f)}{\partial f}hdy\]
\[\delta G[f][h]=\int\frac{\partial g(y,f)}{\partial f}\delta(x-y)dy\]
\[\frac{\delta G[f]}{\delta f(x)}=\frac{\partial g(x,f)}{\partial f} \qquad \blacksquare\]

\[\S\qq{Given}H[f]=\int g(y,f,f')dy\]
show that \[\frac{\delta H[f]}{\delta f(x)}=\frac{\partial g}{\partial f} -\frac{d}{dx}\frac{\partial g}{\partial f'} \quad\text{where}\quad f'=\frac{\partial f}{\partial y}\]
\[\delta H[f][h]=\frac{d}{d\epsilon}H[f+\epsilon h]\Big\vert_{\epsilon=0}\]
\[\delta H[f][h]=\frac{d}{d\epsilon}\int g(y,f+\epsilon h,(f+\epsilon h)')dy\]
\[\delta H[f][h]=\frac{d}{d\epsilon}\int g\left(y,f+\epsilon h,f'+\epsilon h'\right)dy\]
Same trick works \[g(y,f+\epsilon h,f'+\epsilon h')=g(y,f,f')+\frac{1}{1!}\frac{\partial g(y,f,f')}{\partial f}(\epsilon h) + \cdots +\frac{1}{1!}\frac{\partial g(y,f,f')}{\partial f'}(\epsilon h') + \cdots \]
\[\delta H[f][h]=\int\frac{\partial g(y,f,f')}{\partial f}hdy+\int\frac{\partial g(y,f,f')}{\partial f' }h'dy\] Recall \[(uv)'=u'v+uv'\] and find
\[\delta H[f][h]=\int\frac{\partial g(y,f,f')}{\partial f}hdy+\frac{\partial g(y,f,f')}{\partial f'}h\Big \vert_a^b-\int\frac{\partial}{\partial y}\frac{\partial g(y,f,f')}{\partial f'}hdy\]
\[\delta H[f][h]=\frac{\partial g(x,f,f')}{\partial f}+\frac{\partial g(y,f,f')}{\partial f'}\delta(x-y)\Big \vert_a^b-\int\frac{\partial}{\partial y}\frac{\partial g(y,f,f')}{\partial f'}\delta(x-y)dy\]
\[\delta H[f][h]=\frac{\partial g(x,f,f')}{\partial f}-\frac{d}{dx}\frac{\partial g(x,f,f')}{\partial f'} \qquad \blacksquare\]

\[\S\qq{Given}J[f]=\int g(y,f,f',f'')dy\]
show that \[\frac{\delta J[f]}{\delta f(x)}=\frac{\partial g}{\partial f} -\frac{d}{dx}\frac{\partial g}{\partial f'}+\frac{d^2}{dx^2}\frac{\partial g}{\partial f''} \quad\text{where}\quad f''=\frac{\partial^2 f}{\partial y^2}\]
As above \[\delta J[f][h]=\frac{d}{d\epsilon}\int g\left(y,f+\epsilon h,f'+\epsilon h',f'+\epsilon h'\right)dy\]
Focus on \[g(y,f+\epsilon h,f'+\epsilon h',f''+\epsilon h'')= \cdots +\frac{1}{1!}\frac{\partial g(y,f,f',f'')}{\partial f''}(\epsilon h'') + \cdots \]
\[\delta J[f][h]=\int\frac{\partial g(y,f,f',f'')}{\partial f}hdy+\int\frac{\partial g(y,f,f',f'')}{\partial f'}h'dy+\int\frac{\partial g(y,f,f',f'')}{\partial f''}h''dy\] Recall \[(uv')'=u'v'+uv''\] and find the third term becomes
\[\frac{\partial g(y,f,f',f'')}{\partial f''}h'\Big \vert_a^b-\int\frac{\partial}{\partial y}\left[\frac{\partial g(y,f,f',f'')}{\partial f''}\right]h'dy\]
from there find
\[\frac{\partial g(y,f,f',f'')}{\partial f''}h'\Big \vert_a^b-\frac{\partial}{\partial y}\left[\frac{\partial g(y,f,f',f'')}{\partial f''}\right]h\Big \vert_a^b+\int\frac{\partial^2}{\partial y^2}\left[\frac{\partial g(y,f,f',f'')}{\partial f''}\right]hdy\]
hence
\[\delta J[f][h]=\frac{\partial g(x,f,f',f'')}{\partial f}-\frac{d}{dx}\frac{\partial g(x,f,f',f'')}{\partial f'}+\frac{d^2}{dx^2}\frac{\partial g(x,f,f')}{\partial f''} \qquad \blacksquare\]


\section*{Problem 1.4}
Show that \[\frac{\delta\phi(x)}{\delta\phi(y)}=\delta(x-y)\]
and \[\frac{\delta\dot{\phi}(t)}{\delta\phi(t_0)}=\frac{d}{dt}\delta(t-t_0)\]
\[\S\qquad\delta[\phi][h]=\frac{d}{d\epsilon}\left[\phi+\epsilon h\right]=h\]
\[\frac{\delta\phi(x)}{\delta\phi(y)}=\delta(x-y) \qquad \blacksquare\]
\[\S\qquad\delta[\dot{\phi}][h]=\frac{d}{d\epsilon}\left[\dot{\phi}+\epsilon \dot{h}\right]=\dot{h}\]
\[\frac{\delta\dot{\phi}(t)}{\delta\phi(t_0)}=\frac{d}{dt}\delta(t-t_0) \qquad \blacksquare\]


\section*{Problem 1.5}
Given \[V=\frac{\mathcal{T}}{2}\int d^3 x(\nabla\psi)^2\]
and \[T=\frac{\rho}{2}\int d^3 x\left(\frac{\delta \psi}{\delta t}\right)^2\]
The Lagrangian is \[L=T-V\] and the action is \[S=\int_0^\tau Ldt\]

Apply all this to find
\[S=\int_0^\tau dt \int d^3 x\left[\frac{\rho}{2}\left(\frac{\delta \psi}{\delta t}\right)^2 - \frac{\mathcal{T}}{2}(\nabla\psi)^2 \right]\]

Invoke the machinery of functional derivatives
\[\delta S[\psi][h]=\frac{d}{d\epsilon}S[\psi+\epsilon h]\]
Look at the integrand alone
\[\frac{\rho}{2}\left(\frac{\delta (\psi+\epsilon h)}{\delta t}\right)^2 - \frac{\mathcal{T}}{2}\left(\nabla(\psi+\epsilon h)\right)^2\]
Expand
\[\frac{\rho}{2}\left(\frac{\delta \psi}{\delta t}+\epsilon \frac{\delta h}{\delta t}\right)^2 - \frac{\mathcal{T}}{2}\left(\nabla \psi+\epsilon \nabla h\right)^2\]
Compute the derivative with respect to $\epsilon$
\[\rho\frac{\delta \psi}{\delta t}\frac{\delta h}{\delta t} - \mathcal{T}\nabla \psi \nabla h\]
Use the last part of Problem 1.2 to find
\[\delta S[\psi][h]=-\rho\frac{\delta^2 \psi}{\delta t^2} + \mathcal{T}\nabla^2 \psi =0\]
Hence
\[\nabla^2 \psi=\frac{\rho}{\mathcal{T}}\frac{\delta^2 \psi}{\delta t^2} \qquad \blacksquare\]

\section*{Problem 1.6}
\[\qq*{Given}Z_0[J]=\exp\left(-\frac{1}{2}\int d^4 x\, d^4 y\, J(x) \Delta(x-y) J(y)\right)\qq{where}\Delta(x)=\Delta(-x)\]


\[\qq*{Figure the functional derivative}\var Z[J][h]=\dv{\epsilon}Z[J+\epsilon h]\]
Look at the integrand alone
\[(J(x)+\epsilon h) \Delta(x-y) (J(y)+\epsilon h)\]
\[(J(x)J(y)+\epsilon h J(x)+\epsilon h J(y)+\epsilon^2 h^2) \Delta(x-y)\]
Take the derivative with respect to $\epsilon$
\[J(x) \Delta(x-y)h + J(y) \Delta(x-y)h\]
\begin{align*}
    \var{ Z[J][h]} & =-\frac{1}{2}Z_0[J]\left(\int d^4 x\,  J(x) \Delta(x-y)h +\int d^4 y\,J(y) \Delta(x-y)h\right)                    \\
                   & =-\frac{Z_0[J]}{2}\left(\int d^4 x\,  J(x) \Delta(x-y)\delta(x-y) +\int d^4 y\,J(y) \Delta(x-y)\delta(x-y)\right) \\
                   & =-\frac{Z_0[J]}{2}\left(\int d^4 x\,  J(x) \Delta(x-y)\delta(y-x) +\int d^4 y\,J(y) \Delta(x-y)\delta(x-y)\right) \\
                   & =-Z_0[J]\left(\int d^4 y\,J(y) \Delta(y-x)\delta(x-y)\right)                                                      \\
\end{align*}
\[\qq*{Using}\Delta(x)=\Delta(-x)\qand \delta(x-y)=\delta(y-x)\qq{above and changing variables to add the integrals.}\]

\[\fdv{Z[J]}{J[z_1]}=-\left[\int d^4 y\, \Delta(z_1-y)J(y)\right]Z_0[J] \qquad \blacksquare\]


\end{document}
